SeprefUF.thy
@@ -7,12 +7,12 @@ begin
 
   definition "per_init D \<equiv> {(i,i) | i. i\<in>D}"
   definition [simp]: "per_compare R a b \<equiv> (a,b)\<in>R"
-  
+
   definition per_init' :: "nat \<Rightarrow> nat per" where "per_init' n \<equiv> {(i,i) |i. i<n}"
-  
+
   lemma per_init_of_nat_range: "per_init {i. i<N} = per_init' N"
     by (auto simp: per_init_def per_init'_def)
-  
+
   lemma per_init_per[simp, intro!]:
     "part_equiv (per_init D)"
     unfolding per_init_def
@@ -20,30 +20,30 @@ begin
 
   lemma per_init_self: "(a,b)\<in>per_init D \<Longrightarrow> a=b"
     unfolding per_init_def by simp
-  
-  lemma per_union_impl: "(i,j)\<in>R \<Longrightarrow> (i,j)\<in>per_union R a b"  
+
+  lemma per_union_impl: "(i,j)\<in>R \<Longrightarrow> (i,j)\<in>per_union R a b"
     by (auto simp: per_union_def)
 
   lemma per_union_related:
     "part_equiv R \<Longrightarrow> a\<in>Domain R \<Longrightarrow> b\<in>Domain  R \<Longrightarrow> (a,b)\<in>per_union R a b"
     unfolding per_union_def
     by (auto simp: part_equiv_refl)
-    
+
   lemma part_equiv_refl':
     "part_equiv R \<Longrightarrow> x\<in>Domain R \<Longrightarrow> (x,x)\<in>R"
     using part_equiv_refl[of R x] by blast
-        
-  
 
-  sepref_register per_init per_compare per_union
-  
+
+
+  sepref_register per_init per_init' per_compare per_union
+
   lemma per_init_Domain[simp]: "Domain (per_init D) = D"
     by (auto simp: per_init_def)
-  
+
   lemma per_init'_Domain[simp]: "Domain (per_init' N) = {i. i<N}"
     by (auto simp: per_init'_def)
-      
-  
+
+
   lemma per_init'_sepref_rule[sepref_fr_rules]: "(uf_init,RETURN o per_init') \<in> nat_assn\<^sup>k \<rightarrow>\<^sub>a is_uf"
     unfolding per_init'_def
     apply sepref_to_hoare
@@ -54,23 +54,23 @@ begin
     unfolding per_compare_def
     apply sepref_to_hoare
     by sep_auto
-      
+
   lemma per_union_sepref_rule[sepref_fr_rules]: "(uncurry2 uf_union, uncurry2 (RETURN ooo per_union)) \<in>
     [\<lambda>((R,i),j). i\<in>Domain R \<and> j\<in>Domain R ]\<^sub>a is_uf\<^sup>d *\<^sub>a nat_assn\<^sup>k *\<^sub>a nat_assn\<^sup>k \<rightarrow> is_uf"
     unfolding per_compare_def
     apply sepref_to_hoare
     by sep_auto
 
-    
-    
+
+
   definition "abs_test \<equiv> do {
     let u = per_init' (5::nat);
     let u = per_union u 1 2;
     let u = per_union u 2 3;
     RETURN (per_compare u 1 3)
-  }"  
-    
-  sepref_definition abs_test_impl is "uncurry0 abs_test" :: "unit_assn\<^sup>k \<rightarrow>\<^sub>a bool_assn" 
+  }"
+
+  sepref_definition abs_test_impl is "uncurry0 abs_test" :: "unit_assn\<^sup>k \<rightarrow>\<^sub>a bool_assn"
     unfolding abs_test_def
     by sepref
 
